#### { 3n + 2 | n ∈ N }
top-down:
1. n = 2 or
2. n - 3 ∈ S

bottom-up:
1. 2 ∈ S, and
2. if n ∈ S, n + 3 ∈ S

rules-of-inference:
1. 2 ∈ S
2. n ∈ S => (n + 3) ∈ S

#### { 2n + 3m + 1 | n, m ∈ N }
top-down:
1. n = 1, or
2. n - 2 ∈ S, or
3. n - 3 ∈ S

bottom-up:
1. 1 ∈ S, and
2. if n ∈ S, n + 2 ∈ S, and
3. if n ∈ S, n + 3 ∈ S

rules-of-inference:

#### { (n, 2n + 1) | n ∈ N }
top-down:
1. (x, y) = (0, 1), or
2. (x - 1, y - 2) ∈ S

bottom-up:
1. (0, 1) ∈ S, and
2. if (x, y) ∈ S, then (x + 1, y + 2) ∈ S

rule-of-inference

#### { (n, n^2) | n ∈ N } rules 中不要使用平方，提示(n + 1)^2 = n^2 + 2n + 1
top-down:
1. (x, y) = (0, 0), or
2. (x - 1, y - 2sqrt y + 1) ∈ S

bottom-up:
1. (0, 0) ∈ S, and
2. (x + 1, y + 2sqrt y + 1) ∈ S

rule-of-inference:

